Util.thy
@@ -1,0 +1,17 @@
+(* Author: Tobias Nipkow *)
+
+theory Util imports Main
+begin
+
+subsection "From functions to lists"
+
+value "[0 ..< 3]"
+
+value "map f [0 ..< 3]"
+
+definition list :: "(nat \<Rightarrow> 'a) \<Rightarrow> nat \<Rightarrow> 'a list" where
+"list s n = map s [0 ..< n]"
+
+value "list f 3"
+
+end
